examples/mc-logic/arm_multiwordScript.sml
@@ -10,7 +10,7 @@ open HolKernel boolLib bossLib Parse;
 open pred_setTheory res_quanTheory arithmeticTheory wordsLib wordsTheory bitTheory;
 open pairTheory listTheory rich_listTheory relationTheory pairTheory;
 open set_sepTheory set_sepLib progTheory arm_progTheory arm_instTheory arm_progLib;
-open multiwordTheory addressTheory;
+open multiwordTheory arm_evalTheory addressTheory;
 
 (*
   quietdec := false;
