examples/mc-logic/addressScript.sml
@@ -1,157 +1,26 @@
-(* load "wordsLib"; *)
 
 open HolKernel boolLib bossLib Parse;
 open wordsTheory wordsLib bitTheory arithmeticTheory fcpTheory;
+open systemTheory arm_evalTheory;
 
 val _ = new_theory "address";
 
-infix \\ << >>
-
+infix \\ 
 val op \\ = op THEN;
-val op << = op THENL;
-val op >> = op THEN1;
 
 val RW = REWRITE_RULE;
 val RW1 = ONCE_REWRITE_RULE;
 
 
-val aligned_def = Define `aligned (x:word32) = (x && 3w = 0w)`;
+(* definitions *)
 
-val addr32_def = Define `addr32 (x:word30) = (w2w x << 2):word32`;
-val addr30_def = Define `addr30 (x:word32) = ((31 >< 2) x):word30`;
+val CONTAINER_def = Define `CONTAINER x = x:bool`;
+
+(* theorems *)
 
 val ZERO_word30 = store_thm("ZERO_word30",
   ``1073741824w = 0w:word30``,
   SRW_TAC [WORD_ARITH_EQ_ss] []);
-
-val lem = (GEN_ALL o SIMP_RULE std_ss [AND_IMP_INTRO] o
-   Q.DISCH `dimindex (:'b) - 1 = h` o
-   SIMP_RULE (arith_ss++WORD_EXTRACT_ss) [] o
-   Q.DISCH `dimindex(:'b) < dimindex(:'a)` o SPEC_ALL) WORD_w2w_OVER_ADD;
-
-val lower_addr32_ADD = store_thm("lower_addr32_ADD",
-  ``!w x. (1 >< 0) (addr32 x + w) = ((1 >< 0) w):word2``,
-  SRW_TAC [ARITH_ss, WORD_EXTRACT_ss] [lem, addr32_def]);
-
-val addr32_eq_0 = store_thm("addr32_eq_0",
-  ``!x. (1 >< 0) (addr32 x) = 0w:word2``,
-  SRW_TAC [ARITH_ss, WORD_EXTRACT_ss] [addr32_def]);
-
-val addr32_n2w = store_thm ("addr32_n2w", 
-  ``!n. (addr32 (n2w n)  = n2w (4 * n))``,
-  SIMP_TAC (std_ss++WORD_MUL_LSL_ss) [GSYM word_mul_n2w, addr32_def]
-    \\ SRW_TAC [WORD_BIT_EQ_ss] [n2w_def]);
-
-val n2w_and_1 = store_thm("n2w_and_1",
-  ``!n. (n2w n) && 1w = n2w (n MOD 2):'a word``,
-  SIMP_TAC std_ss [(SIMP_RULE std_ss [] o GSYM o Q.SPEC `0`) BITS_ZERO3]
-    \\ SRW_TAC [WORD_BIT_EQ_ss, BIT_ss] [n2w_def]
-    \\ Cases_on `i = 0`
-    \\ SRW_TAC [ARITH_ss] [BIT_def, BITS_ZERO, BITS_COMP_THM2]);
-  
-val n2w_and_3 = store_thm("n2w_and_3",
-  ``!n. (n2w n) && 3w = n2w (n MOD 4):'a word``,
-  SIMP_TAC std_ss [(SIMP_RULE std_ss [] o GSYM o Q.SPEC `1`) BITS_ZERO3]
-    \\ SRW_TAC [WORD_BIT_EQ_ss, BIT_ss] [n2w_def]
-    \\ Cases_on `i = 0` \\ Cases_on `i = 1`
-    \\ SRW_TAC [ARITH_ss] [BIT_def, BITS_ZERO, BITS_COMP_THM2]);
-
-val aligned_MULT = store_thm("aligned_MULT",
-  ``!x y. aligned x ==> aligned (x + 4w * y)``,
-  NTAC 2 Cases
-  \\ REWRITE_TAC [word_add_n2w,word_mul_n2w,aligned_def,n2w_and_3]
-  \\ ONCE_REWRITE_TAC [ADD_COMM] \\ ONCE_REWRITE_TAC [MULT_COMM] 
-  \\ SIMP_TAC std_ss [MOD_TIMES]);
-
-val addr32_and_3w = store_thm("addr32_and_3w",
-  ``!x. (addr32 x) && 3w = 0w``,
-  Cases \\ REWRITE_TAC [addr32_n2w,n2w_and_3]
-  \\ SIMP_TAC std_ss [RW1 [MULT_COMM] MOD_EQ_0]);
-
-val aligned_addr32 = store_thm("aligned_addr32",
-  ``!x. aligned (addr32 x)``,
-  REWRITE_TAC [aligned_def, addr32_and_3w]);
-
-val addr30_n2w = store_thm("addr30_n2w",
-  ``!n. addr30 (n2w n) = n2w (n DIV 4)``,
-  SRW_TAC [SIZES_ss] [addr30_def, word_extract_n2w, BITS_THM]);
-
-val addr30_addr32_ADD = store_thm("addr30_addr32_ADD",
-  ``!x y. addr30 (addr32 x + y) = x + addr30 y``,
-  NTAC 2 Cases
-  \\ REWRITE_TAC [addr30_n2w,addr32_n2w,word_add_n2w]
-  \\ SIMP_TAC std_ss [ONCE_REWRITE_RULE [MULT_COMM] ADD_DIV_ADD_DIV]);
-
-val addr30_addr32_LEMMA = prove(
-  ``!a. (addr30 (addr32 a + 0w) = a) /\ 
-        (addr30 (addr32 a + 1w) = a) /\ 
-        (addr30 (addr32 a + 2w) = a) /\ 
-        (addr30 (addr32 a + 3w) = a)``,
-  SIMP_TAC std_ss [addr30_addr32_ADD,addr30_n2w,WORD_ADD_0]);
-
-val addr30_addr32 = store_thm("addr30_addr32",
-  ``!x. (addr30 (addr32 x) = x) /\
-        (addr30 (addr32 x + 0w) = x) /\ 
-        (addr30 (addr32 x + 1w) = x) /\ 
-        (addr30 (addr32 x + 2w) = x) /\ 
-        (addr30 (addr32 x + 3w) = x)``,
-  REWRITE_TAC
-    [REWRITE_RULE [WORD_ADD_0] addr30_addr32_LEMMA,addr30_addr32_LEMMA]);
-
-val EXISTS_addr30 = store_thm("EXISTS_addr30",
-  ``!x. (x && 3w = 0w) ==> ?y. x = addr32 y``,
-  SRW_TAC [] [addr32_def] \\ Q.EXISTS_TAC `(31 >< 2) x`
-    \\ SRW_TAC [WORD_EXTRACT_ss] []
-    \\ FULL_SIMP_TAC (std_ss++WORD_BIT_EQ_ss) []);
-
-val add32_addr30 = store_thm("addr32_addr30",
-  ``!x. (x && 3w = 0w) ==> (addr32 (addr30 x) = x)``,
-  REPEAT STRIP_TAC \\ IMP_RES_TAC EXISTS_addr30
-    \\ ASM_REWRITE_TAC [addr30_addr32]);
-
-val addr32_ADD = store_thm ("addr32_ADD", 
-  ``!v w. (addr32 (v + w)  = addr32 v + addr32 w)``,
-  NTAC 2 Cases
-  \\ REWRITE_TAC [addr32_n2w,word_add_n2w,LEFT_ADD_DISTRIB]);
-
-val addr32_NEG = store_thm("addr32_NEG",
-  ``!w. addr32 ($- w) = $- (addr32 w)``,
-  Cases \\ REWRITE_TAC [addr32_n2w] 
-  \\ wordsLib.WORD_EVAL_TAC \\ REWRITE_TAC [addr32_n2w]
-  \\ SIMP_TAC (std_ss++wordsLib.SIZES_ss)
-       [n2w_11,LEFT_SUB_DISTRIB,MOD_COMMON_FACTOR]);
-
-val addr32_SUB = store_thm ("addr32_SUB", 
-  ``!v w. (addr32 (v - w)  = addr32 v - addr32 w)``,
-  REWRITE_TAC [word_sub_def,addr32_ADD,addr32_NEG]);
-  
-val addr32_SUC = store_thm("addr32_SUC",
-  ``!p. addr32 (p + 1w) = addr32 p + 4w``,
-  SIMP_TAC std_ss [addr32_ADD,addr32_n2w]);
-
-val addr30_ADD = store_thm("addr30_ADD",
-  ``!x m. addr30 x + n2w m = addr30 (x + n2w (4 * m))``,
-  Cases \\ REWRITE_TAC [addr30_n2w,word_add_n2w]
-  \\ ONCE_REWRITE_TAC [ADD_COMM]
-  \\ SIMP_TAC std_ss [GSYM ADD_DIV_ADD_DIV,AC MULT_COMM MULT_ASSOC]);  
-
-val ADD_LSL = save_thm("ADD_LSL", WORD_ADD_LSL);
-
-val addr32_11 = store_thm("addr32_11",
-  ``!a b. ((addr32 a = addr32 b) = (a = b)) /\ 
-          ((addr32 a = addr32 b + 0w) = (a = b)) /\ 
-          ((addr32 a + 0w = addr32 b) = (a = b)) /\ 
-          ((addr32 a + 0w = addr32 b + 0w) = (a = b)) /\ 
-          ((addr32 a + 1w = addr32 b + 1w) = (a = b)) /\ 
-          ((addr32 a + 2w = addr32 b + 2w) = (a = b)) /\ 
-          ((addr32 a + 3w = addr32 b + 3w) = (a = b))``,
-  SRW_TAC [] [WORD_EQ_ADD_RCANCEL,
-    simpLib.SIMP_PROVE (std_ss++WORD_BIT_EQ_ss) [addr32_def]
-      ``(addr32 a = addr32 b) = (a = b)``]);
-
-val addr32_EQ_0 = store_thm("addr32_EQ_0",
-  ``!a. (addr32 a = 0w) = (a = 0w)``,
-  REWRITE_TAC [SIMP_RULE std_ss [addr32_n2w] (Q.SPECL [`a`,`0w`] addr32_11)]);
 
 val lem = Q.prove(
    `(!a. addr32 a && 1w = 0w) /\
@@ -213,43 +82,11 @@ val addr32_ABSORB_CONST = store_thm("addr32_ABSORB_CONST",
     (addr32 x - 40w = addr32 (x - 10w))``,    
   SIMP_TAC std_ss [addr32_ADD,addr32_SUB,addr32_n2w,WORD_ADD_0]);
 
-val ADDRESS_ROTATE = store_thm("ADDRESS_ROTATE",
-  ``!q:word32 z:word30. q #>> (8 * w2n ((1 >< 0) (addr32 z):word2)) = q``,
-  SIMP_TAC std_ss [addr32_eq_0,word_0_n2w] \\ STRIP_TAC \\ EVAL_TAC);
+val n2w_and_1 = save_thm("n2w_and_1",
+  (SIMP_RULE std_ss [] o SPEC ``1``) WORD_AND_EXP_SUB1);
 
-val addr30_THM = store_thm("addr30_THM",
-  ``!x. addr30 x = n2w (w2n x DIV 4)``,
-  Cases \\ ASM_SIMP_TAC bool_ss [w2n_n2w,LESS_MOD,addr30_n2w]);
-
-val addr32_THM = store_thm("addr32_THM",
-  ``!x. addr32 x = n2w (4 * w2n x)``,
-  Cases \\ ASM_SIMP_TAC bool_ss [w2n_n2w,LESS_MOD,addr32_n2w]);
-
-val aligned_THM = store_thm("aligned_THM",
-  ``!p. aligned p = ?k. p = k * 4w``,
-  SRW_TAC [] [aligned_def] \\ EQ_TAC \\ SRW_TAC [WORD_MUL_LSL_ss] []
-    << [Q.EXISTS_TAC `(31 >< 2) p`, ALL_TAC]
-    \\ FULL_SIMP_TAC (std_ss++WORD_BIT_EQ_ss) []);
-
-val aligned_NEG_lemma = prove(
-  ``!x. aligned x ==> aligned ($- x)``,
-  ASM_SIMP_TAC std_ss  [aligned_THM,w2n_n2w,LESS_MOD]
-  \\ REPEAT STRIP_TAC \\ Q.EXISTS_TAC `n2w (2**30) - k` 
-  \\ ASM_SIMP_TAC (std_ss++WORD_ARITH_EQ_ss) [WORD_RIGHT_SUB_DISTRIB]            
-  \\ ASM_SIMP_TAC (std_ss++WORD_ss) []);
-
-val aligned_NEG = store_thm("aligned_NEG",
-  ``!x. aligned ($- x) = aligned x``,
-  METIS_TAC [aligned_NEG_lemma,WORD_NEG_NEG]);
-
-val aligned_and_1 = store_thm("aligned_and_1",
-  ``!x. aligned x ==> (x && 1w = 0w)``,        
-  REWRITE_TAC [aligned_THM] \\ NTAC 2 STRIP_TAC
-  \\ ASM_REWRITE_TAC [] \\ POP_ASSUM (fn th => ALL_TAC)
-  \\ Q.SPEC_TAC (`k`,`k`) \\ Cases
-  \\ REWRITE_TAC [word_mul_n2w,word_add_n2w,n2w_and_1,n2w_11]
-  \\ REWRITE_TAC [GSYM (EVAL ``2*2``),MULT_ASSOC]
-  \\ SIMP_TAC (std_ss++SIZES_ss) [MOD_EQ_0]);
+val n2w_and_3 = save_thm("n2w_and_3",
+  (SIMP_RULE std_ss [] o SPEC ``2``) WORD_AND_EXP_SUB1);
 
 val aligned_add_1_and_1 = store_thm("aligned_add_1_and_1",
   ``!x. aligned x ==> ~(x + 1w && 1w = 0w)``,        
@@ -274,11 +111,6 @@ val aligned_add_2_and_3 = store_thm("aligned_add_2_and_3",
 val aligned_add_3_and_3 = store_thm("aligned_add_3_and_3",
   ``!x. aligned x ==> (x + 3w && 3w = 3w)``,tac);
 
-val aligned_ADD = store_thm("aligned_ADD",
-  ``!x y. aligned x /\ aligned y ==> aligned (x + y)``,
-  REWRITE_TAC [aligned_THM] \\ REPEAT STRIP_TAC
-  \\ ASM_REWRITE_TAC [GSYM WORD_RIGHT_ADD_DISTRIB] \\ METIS_TAC []);
-  
 val word_arith_lemma1 = store_thm("word_arith_lemma1",
   ``!n m. (n2w n + n2w m = n2w (n + m):'a word) /\
           (x + n2w n + n2w m = x + n2w (n + m):'a word) /\
@@ -309,6 +141,13 @@ val word_arith_lemma4 = store_thm("word_arith_lemma4",
   \\ REWRITE_TAC [GSYM word_sub_def,word_arith_lemma2]
   \\ REPEAT STRIP_TAC \\ Cases_on `n<m` \\ ASM_REWRITE_TAC [word_sub_def]);
 
+val word_arith_lemma5 = store_thm("word_arith_lemma5",
+  ``!x y m n. (x + n2w n = y + n2w m) = 
+              if n < m then (x = y + n2w m - n2w n) else (x + n2w n - n2w m = y)``,
+  ONCE_REWRITE_TAC [GSYM WORD_EQ_SUB_ZERO]
+  \\ SIMP_TAC std_ss [WORD_SUB_PLUS,WORD_SUB_SUB]
+  \\ METIS_TAC [WORD_SUB_PLUS,WORD_ADD_COMM]);
+
 val addr32_ADD_EQ_ZERO_LEMMA = prove(
   ``!x m. 0 < m /\ w2n x + m < dimword (:'a) ==> ~((x:'a word) + n2w m = 0w)``,
   Cases_word
@@ -323,17 +162,52 @@ val addr32_ADD_EQ_ZERO = store_thm("addr32_ADD_EQ_ZERO",
   \\ FULL_SIMP_TAC (bool_ss++SIZES_ss) [w2n_n2w,LESS_MOD,EVAL ``4 * 1073741824``]
   \\ DECIDE_TAC);
 
-val addr32_ADD_AND_EQ_ZERO = store_thm("addr32_ADD_AND_EQ_ZERO",
-  ``!x. ~(addr32 x + 1w && 3w = 0w) /\ ~(addr32 x + 2w && 3w = 0w) /\ ~(addr32 x + 3w && 3w = 0w)``,
-  Cases_word \\ SIMP_TAC std_ss [addr32_n2w,word_add_n2w,n2w_and_3]
-  \\ ONCE_REWRITE_TAC [MULT_COMM] \\ SIMP_TAC std_ss [MOD_TIMES] \\ EVAL_TAC);
+val word_add_and_3w = store_thm("word_add_and_3w",
+  ``!w. (w + n2w n) && 3w = (w + n2w (n MOD 4)) && 3w``,
+  Cases_word \\ SIMP_TAC std_ss [n2w_and_3,word_add_n2w]
+  \\ `n = n DIV 4 * 4 + n MOD 4` by METIS_TAC [DIVISION,EVAL ``0<4``]
+  \\ ONCE_ASM_REWRITE_TAC []  
+  \\ ONCE_REWRITE_TAC [DECIDE ``m + (k + l) = k + (m + l:num)``]
+  \\ SIMP_TAC std_ss [MOD_TIMES]);
 
-(*
+val aligned_CLAUSES = store_thm("aligned_CLAUSES",
+  ``!x a. (aligned (a + 4w * x) = aligned a) /\ (aligned (4w * x + a) = aligned a) /\
+          (aligned (a + x * 4w) = aligned a) /\ (aligned (x * 4w + a) = aligned a) /\
+          (aligned (a + 4w) = aligned a) /\ (aligned (4w + a) = aligned a)``,
+  Cases_word \\ SIMP_TAC std_ss [aligned_def,word_mul_n2w] 
+  \\ ONCE_REWRITE_TAC [word_add_and_3w] \\ ONCE_REWRITE_TAC [WORD_ADD_COMM] 
+  \\ ONCE_REWRITE_TAC [word_add_and_3w] 
+  \\ SIMP_TAC std_ss [MOD_EQ_0,RW1 [MULT_COMM] MOD_EQ_0,WORD_ADD_0]);    
 
-six characters per symbol:
+val NOT_aligned = store_thm("NOT_aligned",
+  ``!a. aligned a ==> ~(aligned (a + 1w)) /\  ~(aligned (a + 2w)) /\ ~(aligned (a + 3w))``,
+  Cases_word \\ SIMP_TAC std_ss [aligned_n2w,word_add_n2w] 
+  \\ ONCE_REWRITE_TAC [MATCH_MP (GSYM MOD_PLUS) (DECIDE ``0<4``)]
+  \\ STRIP_TAC \\ ASM_REWRITE_TAC [ADD] \\ EVAL_TAC);
 
-EVAL ``31**6 < 2**30``      
-*)
+val word32_add_n2w = store_thm("word32_add_n2w",
+  ``!x n. x + (n2w n):word32 = 
+          if n < 2**31 then x + n2w n else x - n2w (2**32 - n MOD 2**32)``,
+  Cases_word \\ STRIP_TAC
+  \\ SIMP_TAC (std_ss++wordsLib.SIZES_ss) [word_sub_def,word_2comp_n2w]
+  \\ Cases_on `n' < 2147483648` \\ ASM_REWRITE_TAC []
+  \\ `n' MOD 4294967296 < 4294967296` by METIS_TAC [arithmeticTheory.DIVISION,EVAL ``0 < 4294967296``]    
+  \\ Cases_on `n' MOD 4294967296 = 0` THENL [
+    ASM_SIMP_TAC (std_ss++wordsLib.SIZES_ss) []
+    \\ ONCE_REWRITE_TAC [GSYM n2w_mod]
+    \\ ASM_SIMP_TAC (std_ss++wordsLib.SIZES_ss) [],
+    `(4294967296 - n' MOD 4294967296) < 4294967296` by DECIDE_TAC    
+    \\ ASM_SIMP_TAC std_ss []
+    \\ `4294967296 - (4294967296 - n' MOD 4294967296) = n' MOD 4294967296` by DECIDE_TAC
+    \\ ONCE_REWRITE_TAC [GSYM n2w_mod]
+    \\ ASM_SIMP_TAC (std_ss++wordsLib.SIZES_ss) []]);
 
+val CONTAINER_IF_T = store_thm("CONTAINER_IF_T",
+  ``!x y z. CONTAINER x ==> ((if x then y else z) = y:'a)``,
+  SIMP_TAC std_ss [CONTAINER_def]);
+
+val CONTAINER_IF_F = store_thm("CONTAINER_IF_F",
+  ``!x y z. CONTAINER ~x ==> ((if x then y else z) = z:'a)``,
+  SIMP_TAC std_ss [CONTAINER_def]);
 
 val _ = export_theory();
